Flapjack.lean
@@ -12,6 +12,7 @@ import Flapjack.PanToCrep
 import Flapjack.Compile
 import Flapjack.Semantics
 import Flapjack.CrepeSemantics
+import Flapjack.CrepeRuntime
 import Flapjack.CrepeCorrectness
 import Flapjack.PanValues
 import Flapjack.PanMemory
